theories/interpreter_ppi.v
@@ -1,7 +1,7 @@
 From Wasm Require Import common properties tactic typing_inversion.
 From Coq Require Import ZArith.BinInt Program.Equality.
 From mathcomp Require Import ssreflect ssrfun ssrnat ssrbool eqtype seq.
-From Wasm Require Export operations host type_preservation type_progress type_checker type_checker_reflects_typing.
+From Wasm Require Export operations host type_preservation type_progress type_checker type_checker_reflects_typing context_inference.
 Require Import BinNat.
 
 Set Implicit Arguments.
@@ -99,17 +99,54 @@ Definition make_ppi_cfg hs s f es ts (Htype: config_typing s f es ts) : res_ppi 
 Definition run_multi_step (fuel: N) hs s f es ts (Htype: config_typing s f es ts) : res_ppi :=
   run_multi_step_ppi fuel (@make_ppi_cfg hs s f es ts Htype).
 
-Print typing.config_typing.
+Definition cl_typing_inf (s: store_record) (f: function_closure): option (cl_type_check_single s f).
+Proof.
+  destruct f as [inst [ts1 ts2] ts bes | tf h]; last first.
+  - apply Some.
+    unfold cl_type_check_single.
+    by apply cl_typing_host.
+  - destruct (inst_typing_inf s inst) as [C | ] eqn:Hinf; last exact None.
+    apply inst_typing_inf_impl in Hinf.
+    destruct (b_e_type_checker (upd_local_label_return C (ts1 ++ ts) [::ts2] (Some ts2)) bes (Tf nil ts2)) eqn:Htypecheck; last exact None.
+    apply b_e_tc_typing in Htypecheck.
+    apply Some.
+    eapply cl_typing_native; by eauto.
+Defined.
 
-Print s_typing.
+Definition cls_typing_inf (s: store_record) (fs: list function_closure) : option (TProp.Forall (cl_type_check_single s) fs).
+Proof.
+  induction fs as [|f fs]; first by apply Some; econstructor.
+  destruct (cl_typing_inf s f) as [clt | ]; last exact None.
+  destruct IHfs as [clts | ]; last exact None.
+  apply Some.
+  by constructor.
+Defined.
 
-Print frame_typing.
-
-Print inst_typing.
+Definition store_typing_inf (s: store_record): option (store_typing s).
+Proof.
+  destruct (cls_typing_inf s s.(s_funcs)) as [clts | ]; last exact None.
+  destruct (all (fun t => tab_agree s t) s.(s_tables)) eqn:Htabagree; last exact None.
+  destruct (all mem_agree s.(s_mems)) eqn:Hmemagree; last exact None.
+  destruct s as [fs tclss mss ?] => /=.
+  by apply Some; split => //.
+Defined.
 
 Definition run_multi_step' (fuel: N) (s: store_record) (f: frame) (bes: list basic_instruction) (ts: result_type) : option res_ppi.
 Proof.
-  remember (b_e_type_checker 
-Admitted.
-
+  destruct (frame_typing_inf s f) as [C | ] eqn:Hftinf; last exact None.
+  destruct (store_typing_inf s) as [Hst | ]; last exact None.
+  destruct (b_e_type_checker (upd_return C None) bes (Tf nil ts)) eqn:Htypecheck; last exact None.
+  apply b_e_tc_typing in Htypecheck.
+  apply frame_typing_inf_impl in Hftinf.
+  apply Some.
+  assert (config_typing s f (to_e_list bes) ts) as Htype.
+  { constructor; first exact Hst.
+    econstructor; first exact Hftinf; eauto.
+    apply ety_a' with (es := (to_e_list bes)); first by apply to_e_list_basic.
+    replace (to_b_list (to_e_list bes)) with bes; first exact Htypecheck.
+    by apply b_e_elim.
+  }
+  exact (run_multi_step fuel tt Htype).
+Defined.
+  
 End Interpreter_PPI_extract.
